New proofs

Graphlib/DFS2.lean
@@ -8,6 +8,8 @@ import Graphlib.FinEnum
 import Graphlib.Basic
 
 
+#eval false < true
+
 set_option trace.split.failure true
 --set_option diagnostics true
 
@@ -25,6 +27,7 @@ structure dfs_state [FinEnum V] [DecidableEq E] [DecidableEq V]
     pathOrder : V → Nat 
     mother : visited → V
     stack : List V
+    terminated : Bool
 
 abbrev dfs_invar_stack_is_visited [FinEnum V] [DecidableEq E] [DecidableEq V]
     (g: WeightedDiGraph V E) (s : dfs_state g):=
@@ -86,7 +89,7 @@ def dfs_step_expand[FinEnum V] [DecidableEq E] [DecidableEq V]
         else 1 + priorState.pathOrder stackHead
         -- priorState.stack.length
       
-      dfs_state.mk new_visited new_order new_mother new_stack
+      dfs_state.mk new_visited new_order new_mother new_stack False
 
 
 lemma dfs_expand_newly_added_are_adjacent --[FinEnum V] [DecidableEq E] [DecidableEq V]
@@ -148,6 +151,7 @@ lemma dfs_expand_keeps_mother_in_visited --[FinEnum V] [DecidableEq E] [Decidabl
 lemma dfs_expand_keeps_mother_ordered --[FinEnum V] [DecidableEq E] [DecidableEq V]
     (g: WeightedDiGraph V E)
     (priorState : dfs_state g)
+    (start : V)
     (stackHead : V)
     (stackTail : List V):
     dfs_invar_mother_is_visited g priorState ∧
@@ -173,6 +177,46 @@ lemma dfs_expand_keeps_mother_ordered --[FinEnum V] [DecidableEq E] [DecidableEq
         --apply maximum_path_order_is_le
         --simp_all
 
+lemma dfs_expand_keeps_on_stack_or_all_neighbours_visited
+    (g: WeightedDiGraph V E)
+    (priorState : dfs_state g)
+    (stackHead : V)
+    (stackTail : List V):
+     dfs_invar_on_stack_or_all_neighbours_visited g priorState
+     ∧ priorState.stack = (stackHead :: stackTail)
+     → dfs_invar_on_stack_or_all_neighbours_visited g
+          (dfs_step_expand g priorState stackHead stackTail)
+          := by
+      intro ⟨ invar_holds_on_prior_state, stack_composition ⟩ 
+      unfold dfs_invar_on_stack_or_all_neighbours_visited
+      intro ⟨ x, x_now_on_stack⟩
+      by_cases x_not_stack_head : x ≠ stackHead
+      · by_cases x_was_not_in_stack_tail_: x ∈ stackTail
+        · left
+          unfold dfs_step_expand
+          simp_all
+        · by_cases x_not_visited : x ∉ priorState.visited
+          · left
+            unfold dfs_step_expand
+            unfold dfs_step_expand at x_now_on_stack
+            simp at x_now_on_stack
+            simp_all
+          · simp_all -- x was visited before and is not on the stack any more
+            right
+            intro y x_adj_y
+            unfold dfs_step_expand
+            simp_all
+            left
+            have x_invar := invar_holds_on_prior_state x
+            simp_all
+      · simp_all
+        right
+        intro y x_adj_y
+        unfold dfs_step_expand
+        simp_all
+        by_cases h : y ∈ priorState.visited
+        · left; exact h
+        · right; exact h
 
 ---------------------------------------------------------------------------------------
 -- run one step of the DFS. Mostly case distinction and running expansion if necessary
@@ -181,11 +225,38 @@ def dfs_step [FinEnum V] [DecidableEq E] [DecidableEq V]
     (priorState : dfs_state g) :
     (dfs_state g) × (Option (Option V)) :=
   match priorState.stack with
-    | [] => (priorState, some none) -- goal not found
+    | [] => ({priorState with terminated := True} , some none) -- goal not found
     | (s :: xs) =>
-    if s = goal then (priorState, some (some s))
+    if s = goal then ({priorState with terminated := True}, some (some s))
     else
       (dfs_step_expand g priorState s xs, none)
+
+
+lemma dfs_step_visited_subset [FinEnum V] [DecidableEq E] [DecidableEq V]
+    (g: WeightedDiGraph V E) (goal : V)
+    (priorState : dfs_state g) :
+    priorState.visited ⊆ (dfs_step g goal priorState).1.visited := by
+    unfold dfs_step
+    split
+    · simp_all
+    split
+    · simp_all
+    unfold dfs_step_expand
+    simp_all
+
+lemma dfs_step_visited_is_smaller_than_V [FinEnum V] [DecidableEq E] [DecidableEq V]
+    (g: WeightedDiGraph V E) (goal : V)
+    (priorState : dfs_state g):
+   (dfs_step g goal priorState).1.visited.card ≤ Fintype.card V := by
+    apply Finset.card_le_univ
+  
+lemma dfs_step_visited_increases[FinEnum V] [DecidableEq E] [DecidableEq V]
+    (g: WeightedDiGraph V E) (goal : V)
+    (priorState : dfs_state g):
+      (dfs_step g goal priorState).1.visited.card ≥ priorState.visited.card := by
+    change   priorState.visited.card ≤ (dfs_step g goal priorState).1.visited.card
+    apply Finset.card_le_card
+    apply dfs_step_visited_subset
 
 ----------
 -- the step also keeps the invariants
@@ -199,12 +270,12 @@ lemma dfs_step_keeps_stack_in_visited --[FinEnum V] [DecidableEq E] [DecidableEq
         intro stack_is_visited_prior 
         unfold dfs_step
         split
-        · simp_all
-          exact stack_is_visited_prior
+        · unfold dfs_invar_stack_is_visited
+          simp_all
         next _ head tail head_tail_compose =>
         split
-        · simp_all
-          exact stack_is_visited_prior
+        · unfold dfs_invar_stack_is_visited
+          simp_all
         apply dfs_expand_keeps_stack_in_visited
         simp_all
         constructor
@@ -252,21 +323,267 @@ lemma dfs_step_keeps_mother_ordered
         apply dfs_expand_keeps_mother_ordered
         simp_all
 
+lemma dfs_step_keeps_on_stack_or_all_neighbours_visited
+    (g: WeightedDiGraph V E)
+    (priorState : dfs_state g):
+    ∀ goal : V,
+     dfs_invar_on_stack_or_all_neighbours_visited g priorState
+     → dfs_invar_on_stack_or_all_neighbours_visited g
+          (dfs_step g goal priorState).fst := by
+        intro goal
+        intro stack_or_neighbour_visited
+        unfold dfs_step
+        split
+        · simp_all
+          exact stack_or_neighbour_visited
+        next _ head tail head_tail_compose => 
+        split
+        · simp_all
+        apply dfs_expand_keeps_on_stack_or_all_neighbours_visited
+        simp_all
+
+
 
 --------------------------------------------------------------------------------------------------
 -- main recursion loop 
 def dfs_recurse[ FinEnum V] [DecidableEq E] [DecidableEq V]
     (g: WeightedDiGraph V E) (goal : V)
-    (priorState : dfs_state g) :
+    (priorState : dfs_state g)
+    (not_terminated : priorState.terminated = False):
     (dfs_state g) × (Option (Option V)) :=
-  let ⟨ nextState, result ⟩ := dfs_step g goal priorState
-  match result with 
-    | none => dfs_recurse g goal nextState
-    | some x => ⟨ nextState, result ⟩ 
-termination_by (Fintype.card V - priorState.visited.card, priorState.stack.length) -- must be a well-founded relation/measure
+  let qq := dfs_step g goal priorState
+  let nextState := qq.fst
+  let result := qq.snd
+  if result_is_none : result = none then 
+    let still_not_termianted : nextState.terminated = False := by
+      unfold nextState
+      unfold result at result_is_none
+      unfold qq at result_is_none ⊢
+      unfold dfs_step at result_is_none ⊢
+      split
+      · simp_all
+      · next _ head tail compose =>
+        simp_all
+        split
+        all_goals
+          simp_all -- one goal vanishes
+        unfold dfs_step_expand
+        simp_all
+    dfs_recurse g goal nextState still_not_termianted
+  else ⟨ nextState, result ⟩ 
+termination_by (¬priorState.terminated, Fintype.card V - priorState.visited.card, priorState.stack.length, goal) -- must be a well-founded relation/measure
 decreasing_by
-  sorry
+  rw [Prod.lex_iff]
+  apply (Classical.or_iff_not_imp_left).mpr
+  simp_all
+  rw [Prod.lex_iff]
+  constructor
+  · simp_all only [result, qq, nextState]
+  apply (Classical.or_iff_not_imp_left).mpr
+  intro visited_not_decreasing
+  simp_all
 
+  --have h1 : Fintype.card V = Fintype.card V - (dfs_step g goal priorState).1.visited.card + priorState.visited.card := by omega
+  have same_visited : (dfs_step g goal priorState).1.visited.card = priorState.visited.card := by
+    have k2 : (dfs_step g goal priorState).1.visited.card ≤ Fintype.card V :=
+      dfs_step_visited_is_smaller_than_V g goal priorState
+    have k3 : (dfs_step g goal priorState).1.visited.card ≥ priorState.visited.card := 
+      dfs_step_visited_increases g goal priorState
+    omega
+  have visited_eq : priorState.visited = (dfs_step g goal priorState).1.visited := by
+    ext a
+    constructor
+    · apply Finset.mem_of_subset
+      apply dfs_step_visited_subset 
+    apply finsetLemma
+    · apply dfs_step_visited_subset 
+    exact same_visited
+
+  constructor
+  · omega
+  · rw [Prod.lex_iff]
+    apply (Classical.or_iff_not_imp_left).mpr
+    unfold dfs_step
+    split
+    · have contra : nextState.terminated = true := by 
+        clear still_not_termianted same_visited 
+        unfold nextState 
+        unfold qq 
+        unfold dfs_step 
+        split
+        · simp_all
+        split
+        · simp_all 
+        unfold dfs_step_expand
+        simp_all
+      rw [contra] at still_not_termianted
+      exact Bool.noConfusion still_not_termianted 
+    split -- style is bad!
+    · next _ head tail compose is_goal =>
+      have contra : nextState.terminated = true := by 
+        clear still_not_termianted same_visited 
+        unfold nextState 
+        unfold qq 
+        unfold dfs_step 
+        split
+        · simp_all
+        split
+        · simp_all
+        unfold dfs_step_expand
+        simp_all
+      rw [contra] at still_not_termianted
+      exact Bool.noConfusion still_not_termianted 
+    next _ head tail compose not_goal =>
+    unfold dfs_step_expand
+    simp_all
+    simp [Nat.add_comm]
+    intro a head_adj_a
+    rw [visited_eq]
+    unfold dfs_step
+    split
+    · simp_all
+    split
+    · simp_all
+    unfold dfs_step_expand
+    simp_all
+    by_cases h : a ∈ (dfs_step g goal priorState).1.visited
+    · left; exact h
+    · right; exact h
+
+--lemma dfs_recurse_keeps_on_stack_or_all_neighbours_visited
+--    (g: WeightedDiGraph V E)
+--    (priorState : dfs_state g)
+--    (not_terminated : priorState.terminated = False):
+--    ∀ goal : V,
+--     dfs_invar_on_stack_or_all_neighbours_visited g priorState
+--     → dfs_invar_on_stack_or_all_neighbours_visited g
+--          (dfs_recurse g goal priorState not_terminated).fst := by
+--      intro goal invar_on_stack_or_all_nei_visited
+--      unfold dfs_recurse
+--      simp
+--      have h := dfs_step_keeps_on_stack_or_all_neighbours_visited g priorState goal
+--      have hh := h invar_on_stack_or_all_nei_visited
+--
+--      split
+--      · next step_returns_none =>
+--        intro a
+--        intro a_visited
+--        have still_not_terminated : (dfs_step g goal priorState).1.terminated = False := by
+--          unfold dfs_step at ⊢ step_returns_none
+--          simp_all
+--          split
+--          · next stack_empty =>
+--            rw [stack_empty] at step_returns_none
+--            simp_all
+--          · simp_all
+--            split
+--            · next head tail compose is_goal =>
+--              rw [compose] at step_returns_none
+--              simp_all
+--            · unfold dfs_step_expand
+--              simp_all
+--        have gg := dfs_recurse_keeps_on_stack_or_all_neighbours_visited g (dfs_step g goal priorState).1 still_not_terminated goal 
+--        have ggg := gg hh
+--        clear gg h hh
+--        unfold dfs_invar_on_stack_or_all_neighbours_visited at ggg
+--        have gggg := ggg ⟨ a, a_visited ⟩
+--        exact gggg
+--
+--        --unfold dfs_invar_on_stack_or_all_neighbours_visited at h
+--        --have hh := h ⟨ a, a_visited⟩ 
+--
+--      · unfold dfs_invar_on_stack_or_all_neighbours_visited at hh
+--        intro a
+--        intro a_visited
+--        have hhh := hh ⟨ a, a_visited ⟩ 
+--        exact hhh
+--termination_by (¬priorState.terminated, Fintype.card V - priorState.visited.card, priorState.stack.length) -- must be a well-founded relation/measure
+--decreasing_by
+--  rw [Prod.lex_iff]
+--  apply (Classical.or_iff_not_imp_left).mpr
+--  simp_all
+--  rw [Prod.lex_iff]
+--  next invar_holds_prior not_none prop2 prop =>
+--  clear prop prop2 not_none
+--  apply (Classical.or_iff_not_imp_left).mpr
+--  intro card_not_less
+--  have visited_is_smaller_than_V : (dfs_step g goal priorState).1.visited.card ≤ Fintype.card V := by
+--    apply Finset.card_le_univ
+--  
+--  have visited_subset : priorState.visited ⊆ (dfs_step g goal priorState).1.visited := by
+--    unfold dfs_step
+--    split
+--    · simp_all
+--    split
+--    · simp_all
+--    unfold dfs_step_expand
+--    simp_all
+--  have visited_increases: (dfs_step g goal priorState).1.visited.card ≥ priorState.visited.card := by
+--    change   priorState.visited.card ≤ (dfs_step g goal priorState).1.visited.card
+--    apply Finset.card_le_card
+--    exact visited_subset
+--
+--  --have h1 : Fintype.card V = Fintype.card V - (dfs_step g goal priorState).1.visited.card + priorState.visited.card := by omega
+--  have same_visited : (dfs_step g goal priorState).1.visited.card = priorState.visited.card := by
+--    omega
+--  have visited_eq : priorState.visited = (dfs_step g goal priorState).1.visited := by
+--    ext a
+--    constructor
+--    · apply Finset.mem_of_subset
+--      exact visited_subset
+--    apply finsetLemma
+--    · exact visited_subset
+--    exact same_visited
+--  constructor
+--  · omega
+--  · rw [Prod.lex_iff]
+--    apply (Classical.or_iff_not_imp_left).mpr
+--    unfold dfs_step
+--    split
+--    · have contra : nextState.terminated = true := by 
+--        clear still_not_termianted same_visited visited_increases
+--        unfold nextState 
+--        unfold qq 
+--        unfold dfs_step 
+--        split
+--        · simp_all
+--        split
+--        · simp_all 
+--        unfold dfs_step_expand
+--        simp_all
+--      rw [contra] at still_not_termianted
+--      exact Bool.noConfusion still_not_termianted 
+--    split -- style is bad!
+--    · next _ head tail compose is_goal =>
+--      have contra : nextState.terminated = true := by 
+--        clear still_not_termianted same_visited visited_increases
+--        unfold nextState 
+--        unfold qq 
+--        unfold dfs_step 
+--        split
+--        · simp_all
+--        split
+--        · simp_all
+--        unfold dfs_step_expand
+--        simp_all
+--      rw [contra] at still_not_termianted
+--      exact Bool.noConfusion still_not_termianted 
+--    next _ head tail compose not_goal =>
+--    unfold dfs_step_expand
+--    simp_all
+--    simp [Nat.add_comm]
+--    intro a head_adj_a
+--    rw [visited_eq]
+--    unfold dfs_step
+--    split
+--    · simp_all
+--    split
+--    · simp_all
+--    unfold dfs_step_expand
+--    simp_all
+--    by_cases h : a ∈ (dfs_step g goal priorState).1.visited
+--    · left; exact h
+--    · right; exact h
 
 --------------------------------------------------------------------------------------------------
 -- initial configuration of the DFS
@@ -277,7 +594,7 @@ def dfs_initial_state [FinEnum V] [DecidableEq E] [DecidableEq V]
   let initialMother : initialVisited → V := fun x => start 
   let initialPathOrder : V → Nat := fun x => 0 
   let initialStack : List V := [start]
-  dfs_state.mk initialVisited initialPathOrder initialMother initialStack
+  dfs_state.mk initialVisited initialPathOrder initialMother initialStack False
 
 
 ----- Proofs that the initial state of the DFS satisfies the invariants
@@ -309,5 +626,12 @@ def dfs[ FinEnum V] [DecidableEq E] [DecidableEq V]
     (g: WeightedDiGraph V E) (start : V) (goal : V):
     (Option (Option V)) :=
   let startState : dfs_state g := dfs_initial_state g start goal
+  let proof : startState.terminated = False := by
+    unfold startState
+    unfold dfs_initial_state
+    simp
 
-  (dfs_recurse g goal startState).2
+
+  (dfs_recurse g goal startState proof).2
+
+
